src/Tactic.v
@@ -1,5 +1,9 @@
 From Coq Require Import ssreflect ssrfun ssrbool.
-From mathcomp Require Import eqtype seq.
+Local Set Warnings "-notation-overridden".
+From mathcomp Require Import eqtype seq ssrnat.
+
+Require Import Lia.
+Require Import Omega.
 
 Ltac rewrite_is_true :=
   repeat match goal with
@@ -30,10 +34,19 @@ Ltac reflect_ne :=
 
 Ltac simpl_seq :=
   repeat match goal with
-         | [ |- context[_ \in (_ :: _)] ] => rewrite in_cons
-         | [ H: ?x::?y \notin ?z |- _ ] =>
+         | [ H: is_true (?x == ?y) |- context[?x \in (?y :: ?l)] ] => rewrite in_cons
+         | [ H: is_true (?y == ?x) |- context[?x \in (?y :: ?l)] ] => rewrite in_cons
+         | [ H: is_true (?x != ?y) |- context[?x \in (?y :: ?l)] ] => rewrite in_cons
+         | [ H: is_true (?y != ?x) |- context[?x \in (?y :: ?l)] ] => rewrite in_cons
+         | [ H: is_true (?x \in ?l) |- context[?x \in (?y :: ?l)] ] => rewrite in_cons
+         | [ H: is_true (?x \notin ?l) |- context[?x \in (?y :: ?l)] ] => rewrite in_cons
+         | [ |- context[?x \in (?x :: ?l)] ] => rewrite in_cons; rewrite eq_refl
+         | [ H: is_true (?x \notin ?y :: ?z) |- _ ] =>
            let Hne := fresh "H" in
            rewrite in_cons in H; move: H; move => /norP [Hne H]
+         | [ H: is_true (?x \notin ?y ++ ?z) |- _ ] =>
+           let Hne := fresh "H" in
+           rewrite mem_cat in H; move: H; move => /norP [Hne H]
          | _ => idtac
          end.
 
@@ -58,7 +71,35 @@ Ltac ssrsubst :=
          | _ => subst
          end.
 
+Ltac remove_SS :=
+  repeat match goal with
+         | [ H: context[?x.+1 == ?y.+1] |- _ ] => rewrite eqSS in H
+         | [ |- context[?x.+1 == ?y.+1] ] => rewrite eqSS
+         end.
+
+Ltac to_coq_nat :=
+  repeat match goal with
+         | [ H: is_true (?x < ?y) |- _ ] => move => /ltP in H
+         | [ |- is_true (?x != ?y) ] => apply /eqP
+         | [ |- is_true (?x == ?y) ] => apply /eqP
+         | [ H: is_true (~~ (?x < ?y)) |- _ ] => rewrite -leqNgt in H; move => /leP in H
+         end.
+
+Ltac intro_ne :=
+  match goal with
+  | [ |- _ <> _ ] => intro
+  | _ => idtac
+  end.
+
+Ltac bigsubst :=
+  subst ; match goal with
+          | [ H1: ?a = Some ?s1, H2: ?a = Some ?s2 |- _ ] => move: (H1); rewrite H2 => [[Heq]]; bigsubst
+          | _ => idtac
+          end.
+
 Ltac simplssr_ := rewrite_is_true; simpl_seq; simpl_bool; simpleq.
 Ltac simplssr := repeat (reflect_ne_in simplssr_).
 Ltac autossr :=
   first [ solve [ simplssr ; intros ; reflect_ne ; ssrsubst ; simplssr ; first [ by auto | divide_hypotheses ; ssrsubst ; simplssr ; by auto ] ] | idtac ].
+
+Ltac liassr := remove_SS ; to_coq_nat ; intros ; intro_ne ; subst ; first [lia | omega ].
